theories/L4_deBruijn/L4_to_L4_1_to_L4_2.v
@@ -116,7 +116,7 @@ Proof using Type.
 Qed.
 
 
-Require Import L6.cps.
+(* Require Import L6.cps. *)
 
 
 
